src/BinEncoders/Env/Common/Transformer.v
@@ -1,0 +1,11 @@
+Set Implicit Arguments.
+
+Section Transformer.
+  Variable B : Type.
+
+  Class Transformer :=
+    { transform : B -> B -> B;
+      transform_id : B;
+      transform_id_pf : forall l, transform transform_id l = l;
+      transform_assoc : forall l m n, transform l (transform m n) = transform (transform l m) n }.
+End Transformer.
