src/BinEncoders/Env/Lib/FixList.v
@@ -1,0 +1,125 @@
+Require Export
+        Coq.Lists.List.
+Require Import
+        Fiat.BinEncoders.Env.BinLib.FixInt
+        Fiat.BinEncoders.Env.Common.Specs
+        Fiat.BinEncoders.Env.Common.Sig.
+
+Set Implicit Arguments.
+
+Section FixListEncoder.
+  Variable size : nat.
+  Variable A B E E' : Type.
+  Variable Eequiv : E -> E' -> Prop.
+  Variable transformer : Transformer B.
+  Variable A_predicate : A -> Prop.
+  Variable A_encode : A -> E -> B * E.
+  Variable A_decoder : decoder Eequiv transformer A_predicate A_encode.
+
+  Definition FixList := { xs : list A | length xs < exp2_nat size }.
+
+  Definition FixList_getlength
+             (ls : FixList) : {n : N | (n < exp2 size)%N}.
+    refine (exist _ (N_of_nat (length (proj1_sig ls))) _).
+    destruct ls as [ xs xs_pf ]. unfold exp2_nat in xs_pf. simpl.
+    rewrite <- Nnat.N2Nat.id. rewrite <- N.compare_lt_iff.
+    rewrite <- Nnat.Nat2N.inj_compare.
+    rewrite <- Compare_dec.nat_compare_lt.
+    eauto.
+  Defined.
+
+  Definition FixList_predicate (len : {n : N | (n < exp2 size)%N}) (l : FixList) :=
+    FixList_getlength l = len /\
+    forall x, In x (proj1_sig l) -> A_predicate x.
+
+  Fixpoint FixList_encode' (xs : list A) (env : E) : B * E :=
+    match xs with
+    | nil => (transform_id (B:=B), env)
+    | x :: xs' => let (b1, env1) := A_encode x env in
+                  let (b2, env2) := FixList_encode' xs' env1 in
+                      (transform b1 b2, env2)
+    end.
+
+  Definition FixList_encode (l : FixList) := FixList_encode' (proj1_sig l).
+
+  Fixpoint FixList_decode' (s : nat) (b : B) (env' : E') : list A * B * E' :=
+    match s with
+    | O => (nil, b, env')
+    | S s' => let (x1, e1) := decode b env' in
+              let (x, b1) := x1 in
+              let (x2, e2) := FixList_decode' s' b1 e1 in
+              let (xs, b2) := x2 in
+              (x :: xs, b2, e2)
+    end.
+
+  Lemma decode'_length :
+    forall len bin env, length (fst (fst (FixList_decode' len bin env))) = len.
+  Proof.
+    induction len; intuition eauto.
+    simpl. destruct (decode bin env) as [[? ?] ?].
+    specialize (IHlen b e). destruct (FixList_decode' len b e) as [[? ?] ?]. simpl. f_equal. eauto.
+  Qed.
+
+  Lemma exp2_nat_nonzero :
+    forall size, exp2_nat size <> O.
+  Proof.
+    assert (forall size, exp2_nat size > O) as lt_pf.
+    intro s. unfold exp2_nat. unfold exp2. rewrite Znat.positive_N_nat.
+    destruct (Pnat.Pos2Nat.is_succ (exp2' s)). rewrite H. omega.
+    intro s. specialize (lt_pf s). omega.
+  Qed.
+
+  Definition FixList_decode (len : nat) (b : B) (env' : E') : FixList * B * E'.
+    refine (exist _ (fst (fst (FixList_decode' (min (pred (exp2_nat size)) len) b env'))) _,
+            snd (fst (FixList_decode' len b env')),
+            snd (FixList_decode' len b env')).
+    rewrite decode'_length.
+    rewrite NPeano.Nat.min_lt_iff.
+    left. unfold lt.
+    rewrite NPeano.Nat.succ_pred; [ | eapply exp2_nat_nonzero ]; eauto.
+  Defined.
+
+  Theorem FixList_encode_correct :
+    forall len,
+      encode_decode_correct Eequiv transformer (FixList_predicate len) FixList_encode (FixList_decode (nat_of_N (proj1_sig len))).
+  Proof.
+    unfold encode_decode_correct, FixList_predicate, FixList_encode, FixList_decode.
+    intros [len len_pf] env env' xenv xenv' [l l_pf] [l' l'_pf] bin ext ext' Eeq Ppred Penc Pdec. simpl in *.
+    inversion Penc; clear Penc; inversion Pdec; clear Pdec.
+    rewrite <- (sig_equivalence _ (fun xs => length xs < exp2_nat size) l l' l_pf l'_pf).
+    assert (min (pred (exp2_nat size)) (N.to_nat len) = N.to_nat len) as pmin.
+    rewrite Min.min_r; eauto. eapply NPeano.Nat.lt_le_pred. unfold exp2_nat.
+    eapply Compare_dec.nat_compare_lt. rewrite <- Nnat.N2Nat.inj_compare. eauto.
+    unfold FixList_getlength in *. rewrite <- sig_equivalence in Ppred. simpl in *.
+    destruct Ppred. subst. rewrite Nnat.Nat2N.id in *.
+    rewrite pmin in *. clear pmin len_pf l_pf.
+    generalize dependent size; generalize dependent env; generalize dependent env';
+      generalize dependent xenv; generalize dependent bin.
+    induction l; simpl in *.
+
+    intros; inversion H0; subst; intuition eauto; rewrite transform_id_pf; eauto.
+
+    intros.
+    specialize (IHl (fun x pf => H4 x (or_intror pf))).
+    specialize (H4 a (or_introl eq_refl)).
+    destruct (A_encode a env) eqn: ?.
+    destruct (decode (transform bin ext) env') as [[? ?] ?] eqn: ?.
+    destruct (FixList_encode' l e) eqn: ?. inversion H0; subst; clear H0.
+    rewrite <- transform_assoc in Heqp0.
+    pose proof (decode_correct (decoder:=A_decoder) env env' _ _ Eeq H4 Heqp Heqp0); clear Eeq H4 Heqp Heqp0.
+    destruct H as [? [? ?]]. subst.
+    destruct (FixList_decode' (length l) (transform b1 ext) e0) as [[? ?] ?] eqn: ?.
+    specialize (IHl b1 xenv e0 e H Heqp1 size0).
+    rewrite Heqp in IHl. simpl in *.
+    assert (length l0 < exp2_nat size0) by omega.
+    intuition. subst. intuition.
+  Qed.
+End FixListEncoder.
+
+Global Instance FixList_decoder A B size len E E' ctxequiv transformer
+       (A_predicate : A -> Prop)
+       (A_encode : A -> E -> B * E)
+       (A_decoder : decoder ctxequiv transformer A_predicate A_encode)
+  : decoder ctxequiv transformer (@FixList_predicate size _ A_predicate len) (FixList_encode transformer A_encode) :=
+  { decode := @FixList_decode size _ _ E E' _ _ _ _ _ (nat_of_N (proj1_sig len));
+    decode_correct := @FixList_encode_correct _ _ _ _ _ _ _ _ _ _ _ }.
